Update Submission.thy

homework/05/Submission.thy
@@ -6,10 +6,36 @@ inductive ls :: "com \<Rightarrow> state \<Rightarrow> state list \<Rightarrow> 
   Skip: "ls SKIP s [] s" |
   Assign: "(v ::= e, s) \<Rightarrow> t \<Longrightarrow> ls (v ::= e) s [] t" |
   Seq: "\<lbrakk>(c1 ;; c2, s) \<Rightarrow> t; ls c1 s xs t'; ls c2 t' ys t\<rbrakk> \<Longrightarrow> ls (c1 ;; c2) s (xs@t'#ys) t" |
+  IfTrue: "\<lbrakk>bval b s; (c1, s) \<Rightarrow> t; ls c1 s xs t\<rbrakk> \<Longrightarrow> ls (IF b THEN c1 ELSE c2) s (s#xs) t" |
+  IfFalse: "\<lbrakk>\<not>bval b s; (c2, s) \<Rightarrow> t; ls c2 s xs t\<rbrakk> \<Longrightarrow> ls (IF b THEN c1 ELSE c2) s (s#xs) t" |
+  WhileTrue: "\<lbrakk> bval b s1; (c, s1) \<Rightarrow> s2; ls (WHILE b DO c) s2 xs s3 \<rbrakk> \<Longrightarrow> ls (WHILE b DO c) s1 (s1#s2#xs) s3" |
+  WhileFalse: "\<not>bval b s  \<Longrightarrow> ls (WHILE b DO c) s [s] s"
+
+(*
+inductive
+  small_step :: "com * state \<Rightarrow> com * state \<Rightarrow> bool" (infix "\<rightarrow>" 55)
+where
+Assign:  "(x ::= a, s) \<rightarrow> (SKIP, s(x := aval a s))" |
+
+Seq1:    "(SKIP;;c\<^sub>2,s) \<rightarrow> (c\<^sub>2,s)" |
+Seq2:    "(c\<^sub>1,s) \<rightarrow> (c\<^sub>1',s') \<Longrightarrow> (c\<^sub>1;;c\<^sub>2,s) \<rightarrow> (c\<^sub>1';;c\<^sub>2,s')" |
+
+IfTrue:  "bval b s \<Longrightarrow> (IF b THEN c\<^sub>1 ELSE c\<^sub>2,s) \<rightarrow> (c\<^sub>1,s)" |
+IfFalse: "\<not>bval b s \<Longrightarrow> (IF b THEN c\<^sub>1 ELSE c\<^sub>2,s) \<rightarrow> (c\<^sub>2,s)" |
+
+While:   "(WHILE b DO c,s) \<rightarrow>
+            (IF b THEN c;; WHILE b DO c ELSE SKIP,s)"
+*)
+
+(*
+Skip: "ls SKIP s [] s" |
+  Assign: "(v ::= e, s) \<Rightarrow> t \<Longrightarrow> ls (v ::= e) s [] t" |
+  Seq: "\<lbrakk>(c1 ;; c2, s) \<Rightarrow> t; ls c1 s xs t'; ls c2 t' ys t\<rbrakk> \<Longrightarrow> ls (c1 ;; c2) s (xs@t'#ys) t" |
   IfTrue: "\<lbrakk>bval b s; (IF b THEN c1 ELSE c2, s) \<Rightarrow> t; ls c1 s xs t\<rbrakk> \<Longrightarrow> ls (IF b THEN c1 ELSE c2) s xs t" |
   IfFalse: "\<lbrakk>\<not>bval b s; (IF b THEN c1 ELSE c2, s) \<Rightarrow> t; ls c2 s xs t\<rbrakk> \<Longrightarrow> ls (IF b THEN c1 ELSE c2) s xs t" |
   WhileTrue: "\<lbrakk> bval b s1; (c, s1) \<Rightarrow> s2; ls (WHILE b DO c) s2 xs s3 \<rbrakk> \<Longrightarrow> ls (WHILE b DO c) s1 (s2#xs) s3" |
   WhileFalse: "\<not>bval b s  \<Longrightarrow> ls (WHILE b DO c) s [] s"
+*)
 
 declare ls.intros[intro]
 declare ls.cases[elim]
@@ -24,14 +50,19 @@ qed auto
 theorem ls_big: "ls c s ss t \<Longrightarrow> (c,s) \<Rightarrow> t"
   by(induction c s ss t rule: ls.induct, auto)
 
+value " ls (SKIP) <> [] <> "
 
 abbreviation "ss_x c s \<equiv> {map (\<lambda>s. s ''x'') ss |ss t . ls c s ss t}"
 values "ss_x (IF Bc True THEN ''x'' ::= N 3 ELSE ''x'' ::= N 1) <>" \<comment>\<open>[0, 3]\<close>
 values "ss_x (WHILE Less (V ''x'') (N 1) DO ''x'' ::= Plus (V ''x'') (N 1)) <>" \<comment>\<open>[0, 0, 1, 1, 1, 1]\<close>
 
+(*mycases*)
+values "ss_x ( ''x'' ::= N 3;; ''x'' ::= N 4) <>"
+
 lemma ls_step: "\<lbrakk>ls c s ss t; c \<noteq> SKIP\<rbrakk> \<Longrightarrow> (case ss of 
   [] \<Rightarrow> (c,s) \<rightarrow> (SKIP,t) 
 | (x#_) \<Rightarrow> \<exists>c'. (c,s) \<rightarrow> (c',x))"
+  nitpick
   sorry
 
 lemma ls_ls: "\<lbrakk>ls c s\<^sub>1 (s\<^sub>2#ss) s\<^sub>3; (c,s\<^sub>1) \<rightarrow> (c',s\<^sub>2)\<rbrakk> \<Longrightarrow> ls c' s\<^sub>2 ss s\<^sub>3"
